
### 2. 

$$
\begin{aligned}
B(t) & = \frac{1}{2} \int [ 1 - e^{-\beta U(y) } ] d^3 y \\
B(t) & =2 \pi \int_0^\infty [ 1 - e^{-\beta U(y)} ] d y \\
B(t) & =2 \pi \int_0^\infty [ 1 - e^{-\beta \alpha y^{-n} } ] d y
\end{aligned}
$$

As suggested by the question, there is a way to massage this integral into a Gamma function. Taking their suggestion, we make the substitution

$$
\begin{aligned}
y & = x^{-1/n} \left( \frac{\alpha}{T} \right)^{1/n} \\
dy & = - \frac{1}{n} x^{-1 - 1/n} \left( \frac{\alpha}{T} \right)^{1/n}  dx
\end{aligned}
$$

and since $x = 0 \leftrightarrow y = \infty$ and $x = \infty \leftrightarrow y = 0$ the integral limits is flipped, and we get a negative sign that cancels with the substitution of $dy$. We get

$$
\begin{aligned}
B(T) = \frac{2 \pi}{n} \left( \frac{\alpha}{T} \right)^{3/n} \int_0^\infty x^{-1 -3/n} ( 1- e^{-x}) dx
\end{aligned}
$$

Integrate by parts

$$
\int_0^\infty x^{-1 -3/n} ( 1- e^{-x}) dx = \left[ \frac{x^{-3/n}}{-3/n} (1 - e^{-x}) \right]_0^\infty + \frac{n}{3} \int_0^\infty x^{-3/n} e^{-x} dx
$$

Let's look at the first term.

- For $x \to \infty$, we have $(1 - e^{-x}) = 1$, and $x^{-3/n} = 0$.

- When $x \to 0$, we have that $x^{-3/n} \to \infty$, but $(1 - e^{-x}) = 0$. The limit still vanishes overall:

$$
\lim_{x \to 0} \frac{1 - e^{-x}}{x^{-3/n}} = \lim_{x \to 0} \frac{x - \frac{1}{2} x^2 + O(x^3)}{x^{-3/n}} = \lim_{x \to 0}\ \left(x^{1 - 3/n}-\frac{1}{2} x^{2-3/n} + O(x^{3 - 3/n}) \right) = 0
$$

as $n > 3$.

We are left with

$$
\int_0^\infty x^{-1 -3/n} ( 1- e^{-x}) dx =  \frac{n}{3} \Gamma(1-3/n)
$$

Using the identity $\Gamma(1 + z) = z \Gamma(z)$, we get

$$
\begin{aligned}
B(T) = - \frac{2 \pi}{n} \left( \frac{\alpha}{T} \right)^{3/n} \Gamma(-3/n)
\end{aligned}
$$

Setting $n=6$, we get

$$
\begin{aligned}
B(T) = \frac{2}{3} \pi^{3/2} \sqrt{ \frac{\alpha}{T} }.
\end{aligned}
$$
<!--stackedit_data:
eyJoaXN0b3J5IjpbLTE0ODQ3MDk3MDVdfQ==
-->