
$$
\begin{ali
\dot{S}_{ij}^{\alpha}&=&-\lambda_{ij}^{\alpha}S_{ij}^{\alpha}&+&\sum_{k}[T_{i,(k\to j)j}^{S,\alpha}-T_{i,j(j\to k)}^{S,\alpha}]\\\dot{I}_{ij}^{\alpha}&=&\lambda_{ij}^{\alpha}S_{ij}^{\alpha}-\gamma_{ij}^{\alpha}I_{ij}^{\alpha}&+&\sum_{k}[T_{i,(k\to j)j}^{I,\alpha}-T_{i,j(j\to k)}^{I,\alpha}]\\\dot{R}_{ij}^{\alpha}&=&\gamma_{ij}^{\alpha}I_{ij}^{\alpha}&+&\sum_{k}[T_{i,(k\to j)j}^{R,\alpha}-T_{i,j(j\to k)}^{R,\alpha}]\\\dot{S}_{i(j\to k)}^{\alpha}&=&-\tau_{i(j\to k)}^{\alpha}S_{i(j\to k)}^{\alpha}&+&T_{i,j(j\to k)}^{S,\alpha}-T_{i,(j\to k)k}^{S,\alpha}\\\dot{I}_{i(j\to k)}^{\alpha}&=&\tau_{i(j\to k)}^{\alpha}S_{i(j\to k)}^{\alpha}-\gamma_{i(j\to k)}^{\alpha}I_{i(j\to k)}^{\alpha}&+&T_{i,j(j\to k)}^{I,\alpha}-T_{i,(j\to k)k}^{I,\alpha}\\\dot{R}_{i(j\to k)}^{\alpha}&=&\gamma_{i(j\to k)}^{\alpha}I_{i(j\to k)}^{\alpha}&+&T_{i,j(j\to k)}^{R,\alpha}-T_{i,(j\to k)k}^{R,\alpha}
$$
<!--stackedit_data:
eyJoaXN0b3J5IjpbLTE2Mzk0NTU2MzNdfQ==
-->